Readme.md
@@ -1,0 +1,9 @@
+Goals:
+
+Complete missing steps
+Figure out use for other direction of correctness proofs?
+Modularize code with classes
+Remove tags
+User types for printing
+Add Parser?
+Add pairs, sums, unit, void, nats, primrec? sructured types?
